libsodium interop for box and secret box

crypto_hst/Hacl.SecretBox.fst
@@ -4,6 +4,7 @@ open FStar.Buffer
 open FStar.HST
 open Hacl.Constants
 open Hacl.Policies
+open Hacl.Cast
 
 (* Module abbreviations *)
 module HS  = FStar.HyperStack
@@ -11,11 +12,29 @@ module B   = FStar.Buffer
 module U8  = FStar.UInt8
 module U32 = FStar.UInt32
 module U64 = FStar.UInt64
+module H8  = Hacl.UInt8
+module H32 = Hacl.UInt32
+module H64 = Hacl.UInt64
 
 (* TODO:
    disjointness clauses
 *)
 
+private val set_zero_bytes:
+  b:uint8_p{length b >= 16} ->
+  Stack unit
+    (requires (fun h -> live h b))
+    (ensures  (fun h0 _ h1 -> live h1 b /\ modifies_1 b h0 h1))
+let set_zero_bytes b =
+  let zero = uint8_to_sint8 0uy in
+  b.(0ul)  <- zero; b.(1ul)  <- zero; b.(2ul)  <- zero; b.(3ul)  <- zero;
+  b.(4ul)  <- zero; b.(5ul)  <- zero; b.(6ul)  <- zero; b.(7ul)  <- zero;
+  b.(8ul)  <- zero; b.(9ul)  <- zero; b.(10ul) <- zero; b.(11ul) <- zero;
+  b.(12ul) <- zero; b.(13ul) <- zero; b.(14ul) <- zero; b.(15ul) <- zero;
+  b.(16ul) <- zero; b.(17ul) <- zero; b.(18ul) <- zero; b.(19ul) <- zero;
+  b.(20ul) <- zero; b.(21ul) <- zero; b.(22ul) <- zero; b.(23ul) <- zero;
+  b.(24ul) <- zero; b.(25ul) <- zero; b.(26ul) <- zero; b.(27ul) <- zero;
+  b.(28ul) <- zero; b.(29ul) <- zero; b.(30ul) <- zero; b.(31ul) <- zero
 
 val crypto_secretbox_detached:
   c:uint8_p ->
@@ -28,9 +47,38 @@ val crypto_secretbox_detached:
     (requires (fun h -> live h c /\ live h mac /\ live h m /\ live h n /\ live h k))
     (ensures  (fun h0 z h1 -> modifies_2 c mac h0 h1 /\ live h1 c /\ live h1 mac))
 let crypto_secretbox_detached c mac m mlen n k =
+  push_frame();
+  let hsalsa_state = create (uint8_to_sint8 0uy) 160ul in
+  let salsa_state = create (uint32_to_sint32 0ul) 32ul in
+  let block0 = sub hsalsa_state 0ul 64ul in
+  let subkey = sub hsalsa_state 64ul 32ul in
+  let block1 = sub hsalsa_state 96ul 64ul in
+  set_zero_bytes block0;
   let mlen = Int.Cast.uint64_to_uint32 mlen in
-  Hacl.Symmetric.Chacha20.xsalsa20_encrypt c k n m mlen;
-  Hacl.Symmetric.Poly1305.poly1305_mac mac c mlen k;
+  let zerobytes = 32ul in
+  let mlen0 =
+    if (U32 (mlen >^ (64ul -^ zerobytes))) then U32 (64ul -^ zerobytes) else mlen in
+  blit m 0ul block0 zerobytes mlen0;
+  Hacl.Symmetric.XSalsa20.hsalsa_init subkey k (sub n 0ul 16ul);
+  Hacl.Symmetric.Salsa20.salsa20_encrypt_body salsa_state
+                                              block1
+                                              subkey
+                                              (uint64_to_sint64 0uL)
+                                              (sub n 16ul 8ul)
+                                              block0
+                                              (U32 (mlen0 +^ zerobytes));
+  (* Hacl.Symmetric.Poly1305.poly1305_init acc r block1; *)
+  blit block1 zerobytes c 0ul mlen0;
+
+  if (U32 (mlen >^ mlen0)) then Hacl.Symmetric.Salsa20.salsa20_encrypt_body salsa_state
+                                                                            (offset c mlen0)
+                                                                            subkey
+                                                                            (uint64_to_sint64 1uL)
+                                                                            (sub n 16ul 8ul)
+                                                                            (offset m mlen0)
+                                                                            (U32 (mlen -^ mlen0));
+  Hacl.Symmetric.Poly1305.poly1305_mac mac c mlen block1;
+  pop_frame();
   0ul
 
 
@@ -46,14 +94,45 @@ val crypto_secretbox_open_detached:
     (ensures  (fun h0 z h1 -> modifies_1 m h0 h1 /\ live h1 m))
 let crypto_secretbox_open_detached m c mac clen n k =
   push_frame();
+  let hsalsa_state = create (uint8_to_sint8 0uy) 160ul in
+  let salsa_state = create (uint32_to_sint32 0ul) 32ul in
+  let tmp_mac = create (uint8_to_sint8 0uy) 16ul in
+  let block0 = sub hsalsa_state 0ul 64ul in
+  let subkey = sub hsalsa_state 64ul 32ul in
+  let block1 = sub hsalsa_state 96ul 64ul in
   let clen = Int.Cast.uint64_to_uint32 clen in
-  let tmp_mac = create (Hacl.Cast.uint8_to_sint8 0uy) 16ul in
-  Hacl.Symmetric.Poly1305.poly1305_mac tmp_mac c clen k;
+  Hacl.Symmetric.XSalsa20.hsalsa_init subkey k (sub n 0ul 16ul);
+  Hacl.Symmetric.Salsa20.salsa20_core block0
+                                      salsa_state
+                                      subkey
+                                      (uint64_to_sint64 0uL)
+                                      (sub n 16ul 8ul)
+                                      64ul;
+  Hacl.Symmetric.Poly1305.poly1305_mac tmp_mac c clen block0;
   assume (Hacl.Policies.declassifiable tmp_mac);
   let verify = cmp_bytes mac tmp_mac 16ul in
-  let z = 
+  let zerobytes = 32ul in
+  (* TODO: report kremlin bug *)
+  let clen0 =
+    if (U32 (clen >^ (64ul -^ zerobytes))) then U32 (64ul -^ zerobytes) else clen in
+  let z =
     if U8 (verify =^ 0uy) then (
-      Hacl.Symmetric.XSalsa20.xsalsa20_encrypt m k n c clen;
+      blit c 0ul block0 zerobytes clen0;
+      Hacl.Symmetric.Salsa20.salsa20_encrypt_body salsa_state
+                                                  block1
+                                                  subkey
+                                                  (uint64_to_sint64 0uL)
+                                                  (sub n 16ul 8ul)
+                                                  block0
+                                                  (U32 (clen0 +^ zerobytes));
+      blit block1 zerobytes m 0ul clen0;
+      if (U32 (clen >^ clen0)) then Hacl.Symmetric.Salsa20.salsa20_encrypt_body salsa_state
+                                                                                (offset m clen0)
+                                                                                subkey
+                                                                                (uint64_to_sint64 1uL)
+                                                                                (sub n 16ul 8ul)
+                                                                                (offset c clen0)
+                                                                                (U32 (clen -^ clen0));
       0x0ul
     )
     else 0xfffffffful in
@@ -72,9 +151,9 @@ val crypto_secretbox_easy:
     (ensures  (fun h0 z h1 -> modifies_1 c h0 h1 /\ live h1 c))
 let crypto_secretbox_easy c m mlen n k =
   let mlen_ = FStar.Int.Cast.uint64_to_uint32 mlen in
-  let c = sub c 0ul mlen_ in
-  let mac = sub c mlen_ 16ul in
-  crypto_secretbox_detached c mac m mlen n k
+  let c'   = sub c 16ul (U32 (mlen_+^16ul)) in
+  let mac  = sub c 0ul 16ul in
+  crypto_secretbox_detached c' mac m mlen n k
 
 
 val crypto_secretbox_open_easy:
@@ -88,6 +167,6 @@ val crypto_secretbox_open_easy:
     (ensures  (fun h0 z h1 -> modifies_1 m h0 h1 /\ live h1 m))
 let crypto_secretbox_open_easy m c clen n k =
   let clen_ = FStar.Int.Cast.uint64_to_uint32 clen in
-  let c = sub c 0ul clen_ in
-  let mac = sub c clen_ 16ul in
-  crypto_secretbox_open_detached m c mac clen n k
+  let c'  = sub c 16ul clen_ in
+  let mac = sub c 0ul 16ul in
+  crypto_secretbox_open_detached m c' mac (U64 (clen -^ 16uL)) n k
